(Mostly) converted Step() to Next()

src/Enumerators/Datatypes.dfy
@@ -1,4 +1,9 @@
+
+include "Enumerators.dfy"
+
 module DatatypeEnumerator {
+
+  import opened Enumerators
 
   datatype E<T> = Done | Next(T, Enum<T>)
   type Enum<T> = () -> E<T>
@@ -19,4 +24,75 @@ module DatatypeEnumerator {
   // function CountupFrom(n: nat): Enum<nat> {
   //   () => Next(n, CountupFrom(n + 1))
   // }
+
+  
+  // Implicit trait approach
+  datatype List<T> = Cons(value: T, tail: List<T>) | Nil {
+    method Enumerator() returns (e: Enumerator<T>) {
+      e := new ListEnumerator(this);
+    }
+
+    function Length(): nat {
+      match this
+      case Cons(_, tail) => 1 + tail.Length()
+      case Nil => 0
+    }
+  }
+
+  class ListEnumerator<T> extends Enumerator<T> {
+
+    var next: List<T>
+
+    constructor(next: List<T>) 
+      ensures Valid()
+      ensures fresh(Repr - {this})
+    {
+      this.next := next;
+
+      enumerated := [];
+      Repr := {this};
+    }
+
+    predicate Valid() 
+      reads this, Repr 
+      ensures Valid() ==> this in Repr 
+      decreases Repr
+    {
+      && this in Repr
+    }
+
+    function Decreases(): nat
+      reads Repr
+      requires Valid()
+    {
+      // This is where I wish I could just say "next" and 
+      // rely on the well-founded ordering.
+      next.Length()
+    }
+
+    predicate method Done() 
+      reads Repr
+      requires Valid()
+      decreases Repr, 0
+      ensures Decreases() == 0 ==> Done()
+    {
+      next.Nil?
+    }
+
+    method Next() returns (element: T)
+      requires Valid()
+      requires !Done()
+      modifies Repr
+      decreases Repr
+      ensures Valid()
+      ensures Repr <= old(Repr)
+      ensures Decreases() < old(Decreases())
+      ensures enumerated == old(enumerated) + [element]
+    {
+      element := next.value;
+      next := next.tail;
+
+      enumerated := enumerated + [element];
+    }
+  }
 }
