src/Enumerators/IteratorAdaptor.dfy
@@ -1,10 +1,12 @@
 
 include "Enumerators.dfy"
+include "../Wrappers.dfy"
 
 module IteratorAdaptorExample {
 
-  import opened Enumerators
 
+  import opened Enumerators
+  import opened Wrappers
   iterator SeqIterator<T(0)>(s: seq<T>) yields (element: T)
     yield ensures elements <= s
     ensures elements == s
@@ -17,7 +19,7 @@ module IteratorAdaptorExample {
     }
   }
 
-  class SeqIteratorEnumerator<T(0)> extends Enumerator<T> {
+  class SeqIteratorEnumerator<T(0)> extends Enumerator<Option<T>> {
 
     const iter: SeqIterator<T>
     var done: bool
@@ -30,18 +32,14 @@ module IteratorAdaptorExample {
       ensures fresh(Repr) 
     {
       iter := new SeqIterator(s);
+      done := false;
       original := s;
       enumerated := [];
       
       new;
-
-      // Calling MoveNext() right away ensures we only enumerate yielded state.
-      var more := iter.MoveNext();
-      done := !more;
       
       Repr := {this, iter} + iter._modifies + iter._reads + iter._new;
       decr := |iter.s| - |enumerated|;
-      assert !done ==> iter.elements < iter.s; 
     }
 
     predicate Valid() reads this, Repr ensures Valid() ==> this in Repr {
@@ -54,8 +52,6 @@ module IteratorAdaptorExample {
       && iter._reads <= Repr
       && iter._new <= Repr
       && (!done ==> iter.Valid())
-      && (!done ==> enumerated + [iter.element] == iter.elements)
-      && (done ==> enumerated == iter.elements)
       && (!done ==> iter.elements < iter.s)
       && decr == |iter.s| - |enumerated|
     } 
@@ -69,7 +65,7 @@ module IteratorAdaptorExample {
       done
     }
 
-    method Step()
+    method Next() returns (element: Option<T>)
       requires Valid()
       requires !Done()
       modifies Repr
@@ -77,38 +73,18 @@ module IteratorAdaptorExample {
       ensures Valid()
       ensures Repr <= old(Repr) 
       ensures Decreases() < old(Decreases())
-      ensures enumerated == old(enumerated) + [old(Current())]
+      ensures enumerated == old(enumerated) + [element]
     {
-      enumerated := enumerated + [Current()];
-
-      var more := iter.MoveNext();
-      done := !more;
       
-      assert iter._new == {};
+      var more := iter.MoveNext();
+      if more {
+        element := Some(iter.element);
+      } else {
+        element := None;
+      }
 
       Repr := {this, iter} + iter._modifies + iter._reads + iter._new;
       decr := |iter.s| - |enumerated|;
-
-      assert this in Repr;
-      assert iter in Repr;
-      assert this !in iter._modifies;
-      assert this !in iter._reads;
-      assert this !in iter._new;
-      assert iter._modifies <= Repr;
-      assert iter._reads <= Repr;
-      assert iter._new <= Repr;
-      assert (!done ==> iter.Valid());
-      assert (!done ==> enumerated + [iter.element] == iter.elements);
-      assert (done ==> enumerated == iter.elements);
-      assert !done ==> iter.elements < iter.s; 
-    }
-
-    function method Current(): T
-      reads this, Repr
-      requires Valid()
-      requires !Done()
-    {
-      iter.element
     }
 
     function Decreases(): nat 
